Existieren die [[Ableitung|Ableitungen]] $u'(x)$ und $v'(x)$ dann gilt f√ºr die Ableitung des Quotienten von $u(x)$ und $v(x)\ne 0$ die Regel:
$$
\left[ \frac{u(x)}{v(x)} \right]'=\frac{u'(x)\cdot v(x)-u(x)\cdot v'(x)}{v(x)^2} \text{ kurz } \left[ \frac{u}{v} \right]' = \frac{u'\cdot v-u\cdot v'}{v^2}
$$
auch geschrieben als
$$
\frac{d}{dx}\left[ \frac{u(x)}{v(x)} \right]=\frac{\frac{d}{dx}[u(x)]\cdot v(x)-u(x)\cdot \frac{d}{dx}[v(x)]}{v(x)^2}
$$

## Beispiel
$$
f(x) = \frac{x^2-x+1}{x-1}
$$
$$
\begin{align}
f'(x) &= \left(\frac{x^2-x+1}{x-1}\right)' \\
&= \frac{(x^2-x+1)'(x-1)-(x^2-x+1)(x-1)'}{(x-1)^2} \\
&= \frac{(2x-1)(x-1)-(x^2-x+1)(1)}{(x-1)^2} \\
&= \frac{2x^2-2x-x+1-x^2+x-1}{(x-1)^2} \\
&= \frac{x^2-2x}{(x-1)^2}
\end{align}
$$
